{% include exercise.md name="Ping-pong" id="1455C" labels="`constructive algorithms` `games` `math`" rating=1100 code="edu/edu99/1455c-ping-pong.kt" %}

Again, it was relatively easy to guess that the answer is $$(x-1, y)$$ but why?

Let's compute $$f'(x, y)$$ for a variant of the game where the first player _can give up his right to serve and loose that first game_.  Clearly $$f'(x, 0) = (x, 0)$$ and $$f'(0, y) = (0, y)$$.  Otherwise as a first player we can:

* hit the ball: $$f'(x, y) = rev(f'(y, x-1))$$ where $$rev(a, b) = (b, a)$$ or
* give up: in which case the second player *must* serve, $$f'(x, y) = f(x, y-1) + (0,1)$$.

Now, based on our intuition we observe that $$f'(x, y) = (x, y)$$ and prove it by induction.

Finally, Alice starts and does not have the option not to serve, hence $$f(x, y) = rev(f'(y, x-1)) = rev(y, x-1) = (x-1, y)$$.
