{% include exercise.md name="Row GCD" id="1459C" also-as="1458A" labels="`math` `number theory`" rating=1600 code="r680-699/r691/1459c-row-gcd.kt" %}

Note that the difference between two numbers must be divisible by their $$gcd$$.  More formally: if $$gcd(x, y) = p$$ then $$abs(x-y) % p == 0$$.

So we can sort the initial numbers, throw away the duplicates and pre-compute $$gcd$$ of all the differences, let's call that $$G$$.  Now for a query of $$b_j$$ we can simply compute the answer as: $$gcd(a_1+b_j, G)$$.

Another way to reason about that is as follows.  We know that $$gcd(x, y) = gcd(x-y, y)$$.  We will want to compute $$gcd(a_1 + b_j, a_2+b_j, \ldots, a_n + b_j)$$.  By subtracting the $$a_1+b_j$$ from all the other terms we get that that formula equals to $$gcd(a_1 + b_j, a_2 - a_1, \ldots a_n - a_1)$$, which equals to: $$gcd(a_1 + b_j, gcd(a_2 - a_1, \ldots a_n - a_1))$$. We an easily see that the second argument does not depend on the queries and so we can precompute it and then answering each query comes down to a single $$gcd$$ of 2 arguments.
