We need to have $$a^2 + b^2 = c^2$$ and $$a^2 - c = b$$.  If we subtract the second equation from the first we get:

$$b^2 + c = c^2 - b \iff b(b+1) = (c-1)c \iff b = c-1$$

Now solving for $$a$$:

$$a^2 - c = b \iff a^2 - (b+1)  = b \iff a^2 = 2b + 1$$

For this to have a solution:

- $$a^2$$ must be odd and so $$a$$ must be odd and
- $$a \neq 1$$.

Any $$a$$ with those two constraints gives a unique solution for $$b$$ and $$c$$ and such that $$b < c < a \le n$$ and so is valid.

So we simply must compute the number of odd numbers $$a > 1$$ such that $$a^2 \le n$$.  Naive solution should be $$O(\sqrt(n))$$ which should be good enough but I did that and got TLE so instead I used binary search to find the answer.
